test/rewrite_search.lean
@@ -55,7 +55,39 @@ begin
   -- perform_nth_rewrite_lhs [bar1] 0,
   -- perform_nth_rewrite_lhs [←bar2] 0,
   -- perform_nth_rewrite_lhs [bar3] 0,
-  rewrite_search_using `search,
+  rewrite_search_using `search {trace:=tt},
+end
+
+private structure cat :=
+  (O : Type)
+  (H : O → O → Type)
+  (i : Π o : O, H o o)
+  (c : Π {X Y Z : O} (f : H X Y) (g : H Y Z), H X Z)
+  (li : Π {X Y : O} (f : H X Y), c (i X) f = f)
+  (ri : Π {X Y : O} (f : H X Y), c f (i Y) = f)
+  (a : Π {W X Y Z : O} (f : H W X) (g : H X Y) (h : H Y Z), c (c f g) h = c f (c g h))
+
+attribute [search] cat.li cat.a
+
+private example (C : cat) (X Y Z : C.O) (f : C.H X Y) (g : C.H Y X) (w : C.c g f = C.i Y) (h k : C.H Y Z) (p : C.c f h = C.c f k) : h = k := 
+begin
+rewrite_search_using `search {trace := tt, trace_rules:=tt},
+perform_nth_rewrite [← C.li Y Z h] 0,
+perform_nth_rewrite [← w] 0,
+perform_nth_rewrite [C.a] 0,
+perform_nth_rewrite [p] 0,
+perform_nth_rewrite [← C.a] 0,
+perform_nth_rewrite [w] 0,
+perform_nth_rewrite [C.li Y Z k] 0,
+-- PROJECT automate this!
+rw [← C.li Y Z h],
+rw [← C.li Y Z k],
+rw [← w],
+rw [C.a],
+rw [C.a],
+rw [p],
 end
 
 end tidy.rewrite_search.testing
+
+
