src/tidy/rewrite_all.lean
@@ -19,27 +19,13 @@ meta def lock_tactic_state {α} (t : tactic α) : tactic α
        end
 
 meta def rewrite_without_new_mvars (r : expr) (e : expr) (cfg : rewrite_cfg := {}) : tactic (expr × expr) :=
-lock_tactic_state $ -- Sorry I don't have a MWE example, but without this natural_transformation.lean fails.
+-- lock_tactic_state $ -- Sorry I don't have a MWE example, but without this natural_transformation.lean fails.
 do n_before ← num_goals,
    (new_t, prf, metas) ← rewrite_core r e cfg,
    try_apply_opt_auto_param cfg.to_apply_cfg metas,
    n_after ← num_goals,
    guard (n_before = n_after),
    return (new_t, prf)
-
-meta def mk_eq_symm_under_binders_aux : expr → (nat → expr) → tactic expr
-| (expr.pi n bi d b) f := expr.lam n bi d <$> mk_eq_symm_under_binders_aux b (λ n, f (n+1) (expr.var n))
-| `(%%a = %%b) e := mk_eq_symm (e 0)
-| _ _ := fail "expression must have the form `Π x y z, a = b`"
-
-meta def mk_eq_symm_under_binders : expr → tactic expr
-| e := do t ← infer_type e, mk_eq_symm_under_binders_aux t (λ _, e)
-
-meta def rewrite_entire (r : (expr × bool)) (e : expr) : tactic (expr × expr) :=
-do let sl := simp_lemmas.mk,
-   r' ← if r.2 then mk_eq_symm_under_binders r.1 else pure r.1,
-   sl ← sl.add r',
-   sl.rewrite e failed `eq semireducible
 
 open tactic.interactive
 
@@ -73,19 +59,41 @@ meta def rewrite_fold_aux {α} (F : expr_lens → expr → α → tactic α) : e
 
 meta def rewrite_fold {α} (F : expr_lens → expr → α → tactic α) (e : expr) (a : α) : tactic α := rewrite_fold_aux F expr_lens.entire e a
 
+-- This is a bit of a hack: we manually inspect the proof that `rewrite_core` produced, and deduce from that whether or not the entire expression was rewritten.
+meta def rewrite_is_of_entire' : expr → bool
+| `(@eq.rec _ %%term %%C %%p _ _) := match p with
+                                     | `(@eq.refl _ %%term') := term = term'
+                                     | _ := ff
+                                     end
+| _ := ff
+meta def rewrite_is_of_entire : expr → bool
+| `(@eq.rec _ %%term %%C %%p _ _) := match C with
+                                     | `(λ p, _ = p) := tt
+                                     | _ := ff
+                                     end
+| _ := ff
+
 meta def rewrite_F (r : expr × bool) (l : expr_lens) (e : expr) (state : list (expr × expr)) : tactic (list (expr × expr)) := 
 do 
+  -- pp_e ← pretty_print e,
+  -- pp_r ← pretty_print r.1,
+  -- tactic.trace ("attempting rewrite on " ++ pp_e ++ " using " ++ pp_r),
   (v, pr) ← rewrite_without_new_mvars r.1 e {symm := r.2, md := semireducible},
+  -- pp_v ← pretty_print v,
+  -- tactic.trace pp_v,
+  -- pp_pr ← pretty_print pr tt,
+  -- tactic.trace pp_pr,
   -- Now we determine whether the rewrite transforms the entire expression or not:
-  (do 
-    (w, qr) ← rewrite_entire r e,
-    let w' := l.replace w,
-    qr' ← l.congr qr,
+  if rewrite_is_of_entire pr then
+  do
+    -- tactic.trace ("rewrite succeeded, complete!"),
+    let w' := l.replace v,
+    qr' ← l.congr pr,
     pure ((w', qr') :: state)
-  ) <|>
-  (do
-    pure (state)
-  )
+  else 
+  do 
+    -- tactic.trace ("rewrite succeeded, tunneling!"),
+    pure state
 
 def remove_adjacent_duplicates {α β} (f : α → β) [decidable_eq β] : list α → list α
 | (x :: y :: t) := if f x = f y then
@@ -95,13 +103,16 @@ def remove_adjacent_duplicates {α β} (f : α → β) [decidable_eq β] : list 
 | [x] := [x]
 | [] := []
 
+
+meta def remove_duplicates {α β} (f : α → β) [decidable_eq β] : list α → list α
+| (x :: t) := x :: (remove_duplicates (t.filter $ λ a, f a ≠ f x))
+| [] := []
+
+
 meta def all_rewrites (r : expr × bool) (e : expr) : tactic (list (expr × expr)) :=
 do 
-   goals ← get_goals,
    results ← rewrite_fold (rewrite_F r) e [],
-   let results : list (expr × expr) := remove_adjacent_duplicates (λ p, p.1) results,
-   set_goals goals,
-   pure results
+   return (remove_adjacent_duplicates (λ p, p.1) results)
 
 -- return a list of (e', prf, n, k) where 
 --   e' is a new expression, 
@@ -112,7 +123,7 @@ meta def all_rewrites_list (rs : list (expr × bool)) (e : expr) : tactic (list 
 do
   results ← rs.mmap $ λ r, all_rewrites r e,
   let results' := results.enum.map (λ p, p.2.enum.map (λ q, (q.2.1, q.2.2, p.1, q.1))),
-  return results'.join
+  return (remove_duplicates (λ t, t.1) results'.join)
 
 meta def perform_nth_rewrite (r : expr × bool) (n : ℕ) : tactic unit := 
 do e ← target,
